src/coq/optimisations/Kildall/valueanalysis.v
@@ -3,14 +3,17 @@ Require Import Vellvm.optimisations.maps.
 
 
 Require Import ZArith List String Omega.
-Require Import Vellvm.Ollvm_ast Vellvm.Classes Vellvm.Util Vellvm.CFGProp Vellvm.CFG.
+Require Import Vellvm.Ollvm_ast Vellvm.Classes Vellvm.Util Vellvm.CFGProp Vellvm.CFG Vellvm.AstLib.
 Require Import Vellvm.optimisations.transform.
 Require Import Vellvm.optimisations.paco_util.
 Require Import Vellvm.optimisations.step_trace.
-Require Import Vellvm.optimisations.EqNat.
+Require Import Vellvm.optimisations.vellvm_tactics.
+
 Require Import Vellvm.optimisations.Kildall.valuedomain.
 Require Import Vellvm.optimisations.Kildall.kildall.
 Require Import Vellvm.optimisations.Kildall.static_eval.
+Require Import Vellvm.optimisations.local_cfg.
+Require Import Vellvm.optimisations.SSA_semantics.
 
 Require Import Vellvm.DecidableEquality.
 Require Import Vellvm.DecidableProp.
@@ -22,13 +25,13 @@ Require Import Vellvm.Effects.
 From mathcomp.ssreflect
      Require Import ssreflect ssrbool seq eqtype ssrnat.
 
-
+Set Implicit Arguments.
 
 Print NODE_SET.
 Module NodeSetForward <: NODE_SET.
-  Definition t := list pc.
-  Definition empty := nil : list pc.
-  Definition add (n: pc) (s: t) : t := n :: s.
+  Definition t := list local_pc.
+  Definition empty := nil : list local_pc.
+  Definition add (n: local_pc) (s: t) : t := n :: s.
 
 
   
@@ -43,8 +46,9 @@ Module NodeSetForward <: NODE_SET.
   Definition code_to_pc (fn:function_id) (bk:block_id) (i:instr_id*instr) : pc := mk_pc fn bk (fst i).
   Definition map_code fn bk (c:code) : seq pc := map (code_to_pc fn bk) c.
   Definition block_to_pc fn (b:block) := map_code fn (blk_id b) (blk_code b) ++ (cons (mk_pc fn (blk_id b) (blk_term_id b)) nil).
-Print block_to_cmd. Print block.
 
+
+  
 Lemma all_node_block : forall code fn n instr,  block_to_cmd code n = Some instr -> In (mk_pc fn (blk_id code) n) (block_to_pc fn code).
 Proof. intros. destruct code. simpl in *. unfold block_to_pc. simpl in *. unfold block_to_cmd in *. simpl in *. unfold blk_term_id in *. simpl in *. destruct blk_term. simpl in *.
        destruct ( decide (i = n)). simpl in *. simpl in *. subst. induction blk_code. simpl in *. eauto. simpl in *. right. eauto. induction blk_code. simpl in *. inversion H. simpl in *. simpl in *. destruct a. simpl in *. destruct (decide (n = i0)). simpl in *. unfold code_to_pc. simpl in *. subst. left. eauto. right. eapply IHblk_code; eauto. Qed.
@@ -64,8 +68,8 @@ Definition def_cfg_to_pc (d:definition cfg) := cfg_to_pc (dc_name (df_prototype 
   Definition mcfg_to_pc (m:mcfg) := flatten (map def_cfg_to_pc (m_definitions m)).  
 
 
-Definition all_nodes (code: mcfg) := mcfg_to_pc code.
-  Definition In (p:pc) (l:t) := In p l.
+Definition all_nodes (code: cfg) : list local_pc := nil.
+  Definition In (p:local_pc) (l:t) := In p l.
   Lemma empty_spec:
     forall n, ~In n empty.
 Proof.
@@ -89,81 +93,27 @@ Proof.
 
 Lemma all_nodes_spec:
     forall code n instr,
-    fetch code n = Some instr -> In n (all_nodes code).
+    local_cfg.fetch code n = Some instr -> In n (all_nodes code).
 Proof.
-  unfold fetch. unfold all_nodes. unfold mcfg_to_pc. simpl in *. unfold def_cfg_to_pc. simpl in *. unfold cfg_to_pc. simpl in *. unfold block_to_pc. simpl in *.
-simpl in *. destruct code. induction m_definitions. simpl in *. intros. destruct n. inversion H. 
 
 
 Admitted.
-
-
-
 
 End NodeSetForward.
 
 Module DS := Dataflow_Solver(VA)(NodeSetForward).
 
 
-Definition block_entry_pc (m:mcfg) (f:function_id) (b:block_id) :=
-  match find_block_entry m f b with
-  | Some (BlockEntry a p) => cons p nil
-                   | None => nil
-  end.
 
-
-Definition next_term (m:mcfg) (f:function_id) (t:terminator) :=
-  match t with
-  | TERM_Ret _ => nil
-  | TERM_Ret_void => nil
-  | TERM_Br _ br1 br2 => (block_entry_pc m f br1) ++ (block_entry_pc m f br2) 
-  | TERM_Br_1 br1 => (block_entry_pc m f br1) 
-  | _ => nil
-  end.
-
-
-
-Definition get_successors (m:mcfg) (p:pc) :=
-  match fetch m p with
-  | Some (Term a) => next_term m (fn p) a
-  | Some (CFG.Step (INSTR_Call (_, ID_Global fid) args)) => match incr_pc m p, find_function_entry m fid  with
-                         | None, None => nil
-                         | Some a, Some (FunctionEntry _ b) => cons a (cons b nil)
-                         | Some a, _ => cons a nil
-                         | None, Some (FunctionEntry _ a) => cons a nil
-                                                
-                         end
-  | Some (CFG.Step a) => match incr_pc m p with
-                         | None => nil
-                         | Some a => cons a nil
-                         end
-  | None => nil 
-  end.
-
-
-
-
-Print instr. Print Expr. Print aval.
-
-Print eval_aenv_expr.
-
-
-Definition transfer' (m:mcfg) (p:pc) (a:aenv) : VA.t :=
-  match fetch m p with
+Definition transfer' (m:cfg) (p:local_pc) (a:aenv) : VA.t :=
+  match local_cfg.fetch m p with
   | Some (Term (TERM_Br _ _ _)) => VA.State (AE.Top_except nil)
   | Some (Term (TERM_Br_1 _)) => VA.State (AE.Top_except nil)
-  | Some (CFG.Step (INSTR_Op (SV o))) => match (pt p) with
+  | Some (CFG.Step (INSTR_Op (SV o))) => match (lpt p) with
                                          | IId id => VA.State (AE.set id (eval_aenv_expr a o) a)
                                          | _ => VA.State a
                                          end
-  
-
-
-
-
-
-  | Some (CFG.Step (INSTR_Call _ _)) => VA.State (AE.Top_except nil)
-  | Some _ => match (pt p) with
+    | Some _ => match (lpt p) with
               | IId id => VA.State (AE.set id (vtop) a)
 
               | _ => VA.State a
@@ -172,7 +122,10 @@ Definition transfer' (m:mcfg) (p:pc) (a:aenv) : VA.t :=
   | None => VA.State a
   end.
 
-Definition transfer (m:mcfg) (p:pc) (v:VA.t)  : VA.t :=
+Print VA.t.
+Print VA.t'.
+
+Definition transfer (m:cfg) (p:local_pc) (v:VA.t)  : VA.t :=
   match v with
   | VA.Bot => VA.Bot
   | VA.State ae => match transfer' m p ae with
@@ -183,118 +136,106 @@ Definition transfer (m:mcfg) (p:pc) (v:VA.t)  : VA.t :=
   end.
 
 
-Definition find_func (m:mcfg) :=
-  match find_function_entry m (Name "main") with
-   | Some (FunctionEntry _ p) => Some p
-   | None => None                
-  end.
 
 
-Definition analyse (m:mcfg) :=
-  match find_func m with
-  | Some start_pc => match (DS.fixpoint m fetch get_successors transfer start_pc (VA.State (AE.Bot))) with
+
+Fixpoint add_multiple_aenv (a:aenv) (l:seq (local_id)) :=
+  match l with
+  | nil => a
+  | hd :: tl => AE.set hd vtop (add_multiple_aenv a tl)
+  end. 
+
+
+       
+Lemma add_multiple_correct : forall l a e r, compare_length l r -> ematch e a ->  ematch ((combine l r) ++ e) (add_multiple_aenv a l) .
+Proof.  induction l. simpl in *. intros. eauto.
+        intros. simpl in *. destruct r. inversion H. simpl in *.
+eapply ematch_update; eauto. constructor. Qed.
+
+
+
+
+Print AE.Bot.
+
+Definition analyse (d:definition cfg) :   PCMap.t DS.L.t :=
+  let c := df_instrs d in
+  match find_block (blks c) (init c) with
+  | None =>  PCMap.init (VA.State (AE.top))
+  | Some block => match (DS.fixpoint c local_cfg.fetch successor_local_pc transfer (mk_localpc (init c) (blk_entry_id block))
+                                     (VA.State(add_multiple_aenv (AE.top) (df_args d)))) with
                      | Some res => res
                      | None => PCMap.init (VA.State (AE.top))
-                     end
-                       
-  | None =>  PCMap.init (VA.State (AE.top))
+                  end
+  end.
+
+       
+Definition analyse_cfg (d:definition cfg) := ((dc_name (df_prototype d)), (analyse d)).
+
+Definition analyse_program (m:mcfg) := map analyse_cfg (m_definitions m).
+
+
+Fixpoint fetch_analysis (p:pc) (s: seq (function_id * PCMap.t DS.L.t)) :=
+  match s with
+  | nil => None
+  | (key, map) :: tl => if eq_dec_function_id (fn p) key then Some (map!!(mk_localpc (bk p) (pt p))) else fetch_analysis p tl
   end.
 
 
-(*
-Definition lookup_env_aenv (e:env) (id:raw_id) : aval :=
-  match lookup_env e id with
-  | None => vbot
-  | Some a => avalue a
-  end.
-
-
-
-(*env - aenv*)
-Inductive vmatch : aval -> aval -> Prop :=
-| vtop_match : forall dval, vmatch dval vtop
-| vval_match : forall dval dval1, dval = dval1 -> vmatch (avalue dval1) (avalue dval).
-
-
-
-
-Definition ematch (e:env) (a:aenv) := forall p, vmatch (lookup_env_aenv e p) (AE.get p a).
-
-Inductive vge: aval -> aval -> Prop :=
-| vge_bot : forall v, vge v vbot
-| vge_val : forall v v1, v = v1 -> vge (avalue v) (avalue v1)
-| vge_top : forall v, vge vtop v.
-
-
-
-
-
-Lemma vmatch_ge:
-  forall v x y, vge x y -> vmatch v y -> vmatch v x.
-Proof.
-  induction 1; intros V. inversion V. subst. eauto. constructor. Qed.
-
-
-
-Lemma ematch_ge:
-  forall  e ae1 ae2,
-  ematch e ae1 -> AE.ge ae2 ae1 -> ematch e ae2.
-Proof. intros. unfold ematch in *. intros. unfold AE.ge in *. specialize (H p).
-       specialize (H0 p). unfold AVal.ge in *. simpl in *. destruct ((lookup_env_aenv e p)); eauto. eapply vmatch_ge; eauto. destruct ( AE.get p ae2); simpl in *; eauto. destruct ( AE.get p ae1); eauto. apply vge_bot. inversion H0. inversion H0. destruct (AE.get p ae1). constructor. constructor. destruct (decide (n = n0)). subst; eauto. simpl in *. inversion H0. inversion H0.
-destruct (AE.get p ae1). constructor. constructor. constructor.
-destruct (AE.get p ae1), ( AE.get p ae2); eauto; inversion H; inversion H0; subst. constructor.
-destruct (decide (n1 = n)). subst. eauto. simpl in *. inversion H5. constructor. 
-destruct ( AE.get p ae2), (AE.get p ae1); try constructor; eauto; try inversion H0; inversion H. Qed.
-
-
-
-Lemma vmatch_false : forall e p, vmatch (lookup_env_aenv e p) AVal.bot -> False.
-Proof. intros. inversion H. Qed.
-
-
-Lemma ematch_update:
-  forall e ae v av r,
-  ematch e ae -> vmatch (avalue v) av -> ematch (add_env r v e) (AE.set r av ae).
-Proof.
-  intros. red. intros. remember ( (lookup_env_aenv (add_env r v e) p)).
- assert  (ae <> AE.Bot -> ~ (AVal.beq av AVal.bot) = true ->
-vmatch a ((if loc_id_eq p r then av else AE.get p ae)) -> vmatch a (AE.get p (AE.set r av ae))).
- intros. unfold is_left in. simpl in *. unfold AE.get, AE.set in *. unfold is_left in *. simpl in *. destruct ae. congruence. destruct ( AVal.beq av AVal.bot). contradiction H2; eauto.
- destruct (AVal.beq av AVal.top) eqn:?. simpl in *.
- rewrite lidTree.grspec. unfold lidTree.elt_eq. 
-destruct ( loc_id_eq p r). constructor. eauto.
-rewrite lidTree.gsspec. unfold lidTree.elt_eq. simpl in *.
-destruct ( loc_id_eq p r). eauto. eauto.
-apply H1. unfold not. intros. subst. unfold ematch in *.
-simpl in *. specialize (H r). inversion H. simpl in *.
-unfold not. intros.  apply AVal.beq_eq in H2.
-subst. simpl in *. inversion H0.
-unfold is_left. simpl in *. subst.
-unfold lookup_env_aenv, add_env, lookup_env in *; simpl in *.
-destruct (AstLib.RawID.eq_dec p r), (loc_id_eq p r); subst; eauto; try contradiction n; eauto.
-Qed.
-
-
-*)
- 
 Inductive sound_stack : mcfg -> stack -> Prop :=
 | nil_stack : forall p, sound_stack p nil
 | kret_stack : forall id m p e k ae
-(AN: (analyse m)!!(mk_pc (fn p) (bk p) (IId id)) = VA.State ae)
+                      (AN: fetch_analysis (mk_pc (fn p) (bk p) (IId id)) (analyse_program m) = Some (VA.State ae))
+                      
 (EM: ematch e ae)  (stk:sound_stack m k),
-    (exists tptr tval, fetch m (mk_pc (fn p) (bk p) (IId id)) = Some (CFG.Step (INSTR_Call tptr tval)) /\incr_pc m (mk_pc (fn p) (bk p) (IId id)) = Some p) -> sound_stack m ((KRet e id p)::k)
+    (exists tptr tval, CFG.fetch m (mk_pc (fn p) (bk p) (IId id)) = Some (CFG.Step (INSTR_Call tptr tval)) /\
+                       incr_pc m (mk_pc (fn p) (bk p) (IId id)) = Some p) -> sound_stack m ((KRet e id p)::k)
+
+                                                                                           
 | kret_void_stack : forall m p e k ae (stk:sound_stack m k),
-    (exists tptr tval id, (analyse m)!!(mk_pc (fn p) (bk p) (IVoid id)) = VA.State ae /\ ematch e ae /\ fetch m (mk_pc (fn p) (bk p) (IVoid id)) = Some (CFG.Step (INSTR_Call tptr tval)) /\
-                          incr_pc m (mk_pc (fn p) (bk p) (IVoid id)) = Some p)  -> sound_stack m ((KRet_void e p)::k).
+    (exists tptr tval id,
+        (fetch_analysis (mk_pc (fn p) (bk p) (IVoid id)) (analyse_program m) = Some (VA.State ae)) /\
+        ematch e ae /\
+        CFG.fetch m (mk_pc (fn p) (bk p) (IVoid id)) = Some (CFG.Step (INSTR_Call tptr tval)) /\
+        incr_pc m (mk_pc (fn p) (bk p) (IVoid id)) = Some p)  -> sound_stack m ((KRet_void e p)::k).
+
+
 
 
 Inductive sound_state : mcfg -> state -> Prop :=
-| sound_state_intro :
-    forall m st  ae
+| sound_state_base :
+    forall m st ae
            (sstack: sound_stack m (stack_of st))
-(AN: (analyse m)!!(pc_of st) = VA.State ae)
-(EM: ematch (env_of st) ae) ,
-      sound_state m st.
+ (AN: fetch_analysis (pc_of st) (analyse_program m) = Some (VA.State ae))
+(EM: ematch (env_of st) ae),  sound_state m st.
+
+
+Lemma analyse_entrypoint : forall m fn0 d0 b0 l, compare_length (df_args d0) l ->
+  find_function m fn0 = Some d0 -> find_block (blks (df_instrs d0)) (init (df_instrs d0)) = Some b0 ->
+  exists ae', fetch_analysis {| fn := fn0; bk := init (df_instrs d0); pt := blk_entry_id b0 |} (analyse_program m) = Some (VA.State ae') /\ ematch  (combine (df_args d0) l) ae'.
+Proof. intros. destruct m. unfold find_function in *. simpl in *. induction m_definitions.
+       simpl in *. inversion H0. simpl in *. unfold is_left in *. simpl in *.
+       unfold find_defn in *. unfold ident_of in *. unfold ident_of_definition in *.
+       unfold ident_of in *. unfold ident_of_declaration in *. simpl in *. destruct a. simpl in *. 
+       destruct (decide (ID_Global (dc_name df_prototype) = ID_Global fn0)). inversion e; subst.
+       inversion H0; subst. simpl in *. destruct ( eq_dec_function_id (dc_name df_prototype) (dc_name df_prototype)).
+       simpl in *. unfold analyse. simpl in *. rewrite H1. simpl.
+
+
+destruct ( DS.fixpoint df_instrs fetch successor_local_pc transfer
+          {| lbk := init df_instrs; lpt := blk_entry_id b0 |}
+          (VA.State (add_multiple_aenv (AE.top) df_args))) eqn:?.
+assert (A: VA.ge t!!({| lbk := init df_instrs; lpt := blk_entry_id b0 |})
+                 (VA.State (add_multiple_aenv (AE.top) df_args))) by (eapply DS.fixpoint_entry; eauto). 
+
+destruct ( t !! {| lbk := init df_instrs; lpt := blk_entry_id b0 |}); simpl in A. inversion A.
+simpl. exists ae. split; eauto. eapply ematch_ge; try eapply A.
+
+assert ((combine df_args l) = (combine df_args l) ++ nil). rewrite cats0. eauto. rewrite H2. eapply add_multiple_correct; eauto. simpl. unfold ematch. unfold lookup_env_aenv. simpl in *. intros. constructor.
+exists (AE.top).  rewrite PCMap.gi. split. eauto. simpl in *. constructor.
+contradiction n; eauto. 
+destruct ( eq_dec_function_id fn0 (dc_name df_prototype)). subst. contradiction n; eauto. eauto. Qed.
+
+
 
 
 
@@ -302,33 +243,29 @@ Inductive sound_state : mcfg -> state -> Prop :=
 Lemma analyse_successor:
   forall m n ae ae' s instr,
     (analyse m)!!n = VA.State ae ->
-    fetch m n = Some instr ->
-    In s (get_successors m n) ->
-    transfer' m n ae = ae' ->
-    VA.ge (analyse m)!!s (transfer m n (VA.State ae)).
-Proof. unfold analyse; intros. unfold find_func in *. simpl in *.
-       unfold find_function_entry in *. simpl in *.
-       destruct ( find_function m (Name "main")) eqn:?.
-       destruct ( find_block (blks (df_instrs d)) (init (df_instrs d))) eqn:?.
-       remember ( (VA.State AE.Bot)) as entry.
-       destruct ( DS.fixpoint m fetch get_successors transfer  {| fn := Name "main"; bk := init (df_instrs d); pt := blk_entry_id b |} entry) eqn:?.
-       assert (A: VA.ge t !! s (transfer m n (t !!n))).
-       eapply DS.fixpoint_solution; eauto with coqlib. intros.
-       unfold transfer. apply DS.L.eq_refl. rewrite H in A.
-       unfold transfer in A. unfold transfer in H2. rewrite H2 in A.
-       rewrite H2. unfold transfer.  eauto. simpl in *.
-       destruct (transfer' m n ae). eauto. apply AE.ge_top. rewrite H2.
-       simpl in *. destruct ae'.  eauto. eapply AE.ge_top. simpl in *.
-       rewrite H2. destruct ae'. simpl in *. eauto. eapply AE.ge_top. Qed.
-
-
+    fetch (df_instrs m) n = Some instr ->
+    In s ( successor_local_pc (df_instrs m) n) ->
+    transfer' (df_instrs m) n ae = ae' ->
+    VA.ge (analyse m)!!s (transfer (df_instrs m) n (VA.State ae)).
+Proof. unfold analyse; intros.
+       destruct (find_block (blks (df_instrs m)) (init (df_instrs m))) eqn:?.
+       remember (VA.State AE.Bot) as entry.
+       
+       destruct ( DS.fixpoint (df_instrs m) fetch successor_local_pc transfer
+        {| lbk := init (df_instrs m); lpt := blk_entry_id b |}
+        (VA.State (add_multiple_aenv AE.top (df_args m)))) eqn:?.
+        assert (A: VA.ge t !! s (transfer (df_instrs m) n (t !!n))).
+        eapply DS.fixpoint_solution; eauto with coqlib. intros. unfold transfer. simpl. eauto.
+        rewrite H in A. unfold transfer in A. simpl in *. rewrite H2 in A. rewrite H2.
+        eauto. simpl in *. destruct ( transfer' (df_instrs m) n ae). eauto. eapply AE.ge_top.
+        unfold transfer. simpl in *. rewrite H2. simpl in *. destruct ae'. eauto. eapply AE.ge_top. Qed.
 
 Lemma analyse_succ:
   forall e f n ae instr s ae',
   (analyse f)!!n = VA.State ae ->
-  fetch f n = Some instr ->
-  In s (get_successors f n) ->
-  transfer' f n ae = VA.State ae' ->
+  fetch (df_instrs f) n = Some instr ->
+  In s ( successor_local_pc (df_instrs f) n) ->
+  transfer' (df_instrs f) n ae = VA.State ae' ->
   ematch e ae' ->
   exists ae'',
      (analyse f)!!s = VA.State ae''
@@ -339,71 +276,166 @@ Proof. intros. generalize H; intros. eapply analyse_successor in H4; eauto.
        split. auto. eapply ematch_ge; eauto. Qed. 
 
 
-Lemma sound_succ_state:
-  forall pc ae instr f s pc' e' ae',
-    (analyse f)!!pc = VA.State ae  ->
-    fetch f pc = Some instr -> In pc' (get_successors f pc) ->
-    transfer' f pc ae = VA.State ae' ->
-ematch e' ae' -> sound_stack f s ->
-  sound_state f (pc', e', s).
-Proof.
-  intros. generalize H. intros. eapply analyse_succ in H5; eauto.
-  generalize H5. intros (aea' & aef). destruct aef.
-  simpl in *. inversion H5. destruct H8. simpl in *. econstructor; eauto. Qed.
 
 
-Lemma unfold_fetch : forall m fn0 d bk0 b id  pt0 instr
-  (Heqo : find_function m fn0 = Some d)
-  (Heqo0 : find_block (blks (df_instrs d)) bk0 = Some b)
-  (Heqo1 : block_to_cmd b id = Some (instr, pt0)),
-  fetch m {| fn := fn0; bk := bk0; pt := id|} = Some instr.
-Proof. intros. unfold fetch. simpl in *. rewrite Heqo. rewrite Heqo0. rewrite Heqo1. eauto.
-Qed.
+Definition find_block_pc (m:mcfg) (fn:function_id) (bk:block_id) :=
+  match CFG.find_block_entry m fn bk with
+  | None => nil
+  | Some (BlockEntry _ pc) => cons pc nil
+  end.
+
+                                   
+Definition successor_pc (m:mcfg) (p:pc) :=
+  match CFG.fetch m p with
+  | None => nil
+  | Some (Term t) => match t with
+                     | TERM_Br_1 br => find_block_pc m (fn p) br
+                     | TERM_Br _ br1 br2 => (find_block_pc m (fn p) br1) ++ (find_block_pc m (fn p) br2)
+                     | _ => nil
+                     end
+                         
+  | Some (CFG.Step ins) => match incr_pc m p with
+                                              | Some res => cons res nil
+                                              | None => nil
+                                              end
+                     
+  end.
 
 
-Hint Resolve unfold_fetch.
+Print successor_local_pc.
 
-
-
-Lemma unfold_instr : forall m fn0 d b id instruction pt0 bk0 (Heqo : find_function m fn0 = Some d)
- ( Heqo0 : find_block (blks (df_instrs d)) bk0 = Some b)
-  (Heqo1 : block_to_cmd b id = Some (CFG.Step instruction, Some pt0)),
-  In {| fn := fn0; bk := bk0; pt := pt0 |}
-    (get_successors m {| fn := fn0; bk := bk0; pt := id |}).
-Proof. intros. unfold get_successors. simpl in *. rewrite Heqo. rewrite Heqo0.
-       rewrite Heqo1. destruct instruction; simpl in *; eauto. destruct fn.
-       destruct i. simpl in *. destruct ( find_function_entry m id0) eqn:?.
-       destruct f. simpl in *. eauto. simpl in *. eauto. simpl in *.
-       eauto. Qed.
-Hint Resolve unfold_instr.
-
-
-Lemma transfer_add :
-forall m fn0 d bk0 b ae op pt0 id, 
-find_function m fn0 = Some d ->
-find_block (blks (df_instrs d)) bk0 = Some b ->
-block_to_cmd b (IVoid id) = Some (CFG.Step (INSTR_Op op), Some pt0) ->
-transfer' m {| fn := fn0; bk := bk0; pt := IVoid id |} ae = VA.State ae.
-Proof. intros. unfold transfer'.
-       simpl in *. rewrite H. rewrite H0.
-       rewrite H1. destruct op; simpl in *. destruct e; eauto. Qed.
-Hint Resolve transfer_add.
+Print find_function. Print pc_to_local_pc.
+Print block.
+Lemma find_block_pc_equiv : forall d bk b, find_block (blks (df_instrs d)) bk = Some b -> (blk_id b) = bk.
+Proof. intros. destruct d. simpl in *. destruct df_instrs. simpl in *. induction blks. simpl in *. inversion H.
+simpl in *.  destruct ( decide (blk_id a = bk)). inversion H. subst. simpl in *. eauto. simpl in *. eapply IHblks.
+destruct blks. simpl in *. eauto. simpl in *. eapply H. Qed. 
 
 
 
+       
+Lemma successor_pc_to_local : forall pc pc' m d, In pc' (successor_pc m pc) -> find_function m (fn pc) = Some d -> In (pc_to_local_pc pc') (successor_local_pc (df_instrs d) (pc_to_local_pc pc)).
+Proof. intros. unfold successor_pc in *. simpl in *. unfold successor_local_pc in *.
+       unfold CFG.fetch in *. simpl in *. destruct pc, pc'. simpl in *.
+       unfold pc_to_local_pc in *. simpl in *.
+       unfold cfg_to_cmd. simpl in *. destruct (find_function m fn) eqn:?.
+       inv H0. clear H0.
+       destruct ( find_block (blks (df_instrs d)) bk) eqn:?.
+       destruct ( block_to_cmd b pt) eqn:?. simpl in *. destruct p.
+       simpl in *. destruct c. simpl in *. destruct o. simpl in *.
+       inversion H. inversion H0; subst. left. eauto. inversion H0.
+       simpl in *. inversion H. simpl in *. destruct t; simpl in *; try inv H.
+       unfold find_block_entry in *. simpl in *. unfold find_block_pc in *.
+       simpl in *. unfold CFG.find_block_entry in *. simpl in *.
+       rewrite Heqo in H.
+       destruct (find_block (blks (df_instrs d)) br1) eqn:?, (find_block (blks (df_instrs d)) br2) eqn:?; simpl in *; unfold blk_entry_pc in *; simpl in *; unfold blk_entry_id in *; simpl in *.
+       inversion H. inversion H0; subst; clear H0. simpl. left.
+       eapply find_block_pc_equiv in Heqo2. subst.  eauto. inversion H0.
+       inversion H1; subst. eapply find_block_pc_equiv in Heqo3. subst.
+       eauto. inversion H1. inversion H. inversion H0. subst. simpl in *.
+       eapply find_block_pc_equiv in Heqo2. subst. eauto. inversion H0.
+       inversion H. inversion H0. subst. eapply  find_block_pc_equiv in Heqo3.
+       subst. eauto. inversion H0. inversion H.
+       unfold find_block_pc in *. unfold find_block_entry. unfold CFG.find_block_entry in *.
+       simpl in *. rewrite Heqo in H. destruct (find_block (blks (df_instrs d)) br) eqn:?.
+       simpl in *. inversion H. inversion H0. subst. eapply find_block_pc_equiv in Heqo2.
+       subst. eauto. inversion H0. simpl in *. eauto. simpl in *. eauto.
+       simpl in *. eauto. simpl in *. inversion H. Qed.
 
 
-Lemma block_implies_successor : forall m fn0 d0 bk0 b0 id x x0 pt0,
-find_function m fn0 = Some d0 -> find_block (blks (df_instrs d0)) bk0 = Some b0 -> 
-block_to_cmd b0 id =
-Some (CFG.Step (INSTR_Call x x0), Some pt0) -> In  (mk_pc fn0 bk0 pt0) (get_successors m (mk_pc fn0 bk0 id)).
-Proof. intros. unfold get_successors. simpl in *.
-       rewrite H. rewrite H0. rewrite H1. destruct x.
-       destruct i. simpl in *. unfold find_function_entry in *.
-       simpl in *. destruct (find_function m id0) eqn:?.
-       destruct ( find_block (blks (df_instrs d)) (init (df_instrs d))) eqn:?.
-       simpl in *. eauto. simpl in *. eauto. simpl in *. eauto.
-       simpl in *. eauto.  Qed.
-     Hint Resolve block_implies_successor.
 
-               
+
+
+
+Lemma fetch_local_analysis : forall p m ae d, fetch_analysis p (analyse_program m) = Some (VA.State ae) ->
+                                              find_function m (fn p) = Some d ->
+                                              ((analyse d) !!(mk_localpc (bk p) (pt p))) = VA.State ae.
+Proof. intros. destruct m. simpl in *. unfold analyse_program in *. simpl in *. 
+       destruct d. simpl in *. destruct p. simpl in *. destruct df_instrs. simpl in *.
+       induction m_definitions. unfold find_function in *. simpl in *. inversion H0.
+       simpl in *. unfold find_function in H0. simpl in *. unfold is_left in *. simpl in *. unfold find_defn in H0.
+       simpl in *. unfold ident_of in *. simpl in *. unfold ident_of_definition in *. destruct a. simpl in *.
+       destruct ( decide (ident_of df_prototype0 = ID_Global fn)). unfold ident_of in *.
+       simpl in *. unfold ident_of_declaration in *. simpl in *. inversion e. subst.
+       destruct ( eq_dec_function_id (dc_name df_prototype0) (dc_name df_prototype0)). simpl in *.
+       inversion e; clear e. clear e0. inversion H; inversion H0; subst. clear H0.
+       clear H. eauto. contradiction n; eauto. unfold ident_of in *. simpl in *.
+       unfold ident_of_declaration in *. simpl in *. destruct ( eq_dec_function_id fn (dc_name df_prototype0)).
+       inversion H; subst. contradiction n; eauto. eapply IHm_definitions in H.
+       eapply H. clear  IHm_definitions. clear H. clear n. clear n0. destruct m_definitions.
+       simpl in *. eauto. eauto. Qed.
+
+
+Lemma fetch_to_local_fetch : forall m pc instr d, CFG.fetch m pc = Some instr -> find_function m (fn pc) = Some d -> fetch (df_instrs d) (pc_to_local_pc pc) = Some instr.
+Proof. intros. unfold CFG.fetch in *. simpl in *.
+       destruct pc. simpl in *. rewrite H0 in H.
+       unfold fetch. unfold pc_to_local_pc. simpl in *.
+       unfold cfg_to_cmd. simpl in *.
+       destruct ( find_block (blks (df_instrs d)) bk) eqn:?; eauto. Qed.
+
+Lemma pc_equiv : forall m pc' fn1 bk1 pt1,  In pc' (successor_pc m {| fn := fn1; bk := bk1; pt := pt1 |}) -> (fn pc') = fn1.
+Proof. intros. destruct pc'.  simpl in *. unfold successor_pc in *. simpl in *.
+       destruct (find_function m fn1) eqn:?; simpl in *.
+       destruct (find_block (blks (df_instrs d)) bk1) eqn:?; simpl in *.
+       destruct (block_to_cmd b pt1) eqn:?; simpl in *.
+       destruct p. simpl in *. destruct c. simpl in *. destruct o. simpl in *. inversion H.
+       inversion H0. subst; eauto. inversion H0. simpl in *. inversion H.
+       destruct t; simpl in *; try inversion H. unfold find_block_pc in *.
+       unfold CFG.find_block_entry in *. simpl in *. rewrite Heqo in H.
+       destruct (find_block (blks (df_instrs d)) br1) eqn:?,
+                (find_block (blks (df_instrs d)) br2) eqn:?; simpl in *;
+         unfold blk_entry_pc in *; simpl in *; try inversion H; try inversion H0; subst; eauto.
+       inversion H1; subst; eauto. inversion H1. unfold find_block_pc in *.
+       unfold CFG.find_block_entry in *; simpl in *. rewrite Heqo in H.
+       destruct (find_block (blks (df_instrs d)) br) eqn:?; simpl in *. inversion H; eauto.
+       inversion H0; subst; eauto. inversion H0. inversion H. inversion H. inversion H. inversion H. Qed.
+
+
+
+
+
+
+Lemma fetch_analysis_equiv : forall m fn d bk0 pt0 aef,
+find_function m fn = Some d ->
+ (analyse d) !! {| lbk := bk0; lpt := pt0 |} = VA.State aef ->
+fetch_analysis {| fn := fn; bk := bk0; pt := pt0 |} (analyse_program m) = Some (VA.State aef).
+Proof. intros. destruct m. simpl in *. unfold find_function in *.
+       simpl in *. unfold find_defn in *. simpl in *. unfold ident_of in *.
+       simpl in *. unfold ident_of_definition in *. simpl in *.
+       induction m_definitions. simpl in *. inversion H.
+       simpl in *. unfold is_left in *. unfold ident_of in *.
+       unfold ident_of_declaration in *.
+       destruct a. simpl in *. destruct (decide (ID_Global (dc_name df_prototype) = ID_Global fn)).
+       simpl in *. inversion H. subst. clear H. inversion e. subst. simpl in *.
+       destruct ( eq_dec_function_id (dc_name df_prototype) (dc_name df_prototype)). simpl in *.
+       rewrite H0. eauto. contradiction n; eauto. destruct ( eq_dec_function_id fn (dc_name df_prototype)).
+       subst. contradiction n; eauto. eapply IHm_definitions in H.
+       destruct m_definitions. simpl in *. eauto. simpl in *. eauto. Qed.
+
+
+
+
+
+
+
+       
+Lemma sound_succ_state: forall m d pc ae instr s pc' e' ae',
+fetch_analysis pc (analyse_program m) = Some (VA.State ae) ->
+CFG.fetch m pc = Some instr -> 
+In pc' (successor_pc m pc) ->
+find_function m (fn pc) = Some d ->
+transfer' (df_instrs d) (pc_to_local_pc pc) ae = VA.State ae' ->
+ematch e' ae' -> sound_stack m s ->
+sound_state m (pc', e', s)
+.
+Proof. intros. dupl H1. eapply successor_pc_to_local in H6; eauto. 
+dupl H.
+eapply fetch_local_analysis in H; eauto.
+dupl H0. eapply fetch_to_local_fetch in H8; eauto.
+unfold pc_to_local_pc in *. simpl in *. eapply analyse_succ in H; eauto.
+generalize H. intros (aef & aes'). destruct aes'. simpl in *.
+destruct pc. simpl in *. dupl H1. eapply pc_equiv in H11. destruct pc'. simpl in *. subst.
+econstructor; simpl; eauto. eapply fetch_analysis_equiv; eauto. Qed.
+
+
+
