src/coq/optimisations/SSA_semantics.v
@@ -3,7 +3,7 @@ Require Import Vellvm.Ollvm_ast Vellvm.Classes Vellvm.Util Vellvm.CFGProp Vellvm
 Require Import Vellvm.optimisations.transform.
 Require Import Vellvm.optimisations.paco_util.
 Require Import Vellvm.optimisations.step_trace.
-Require Import Vellvm.optimisations.EqNat.
+Require Import Vellvm.optimisations.vellvm_tactics.
 
 Require Import Vellvm.DecidableEquality.
 Require Import Coq.Logic.FunctionalExtensionality.
@@ -12,7 +12,7 @@ Require Import Vellvm.Memory.
 Require Import Vellvm.Effects.
 From mathcomp.ssreflect
      Require Import ssreflect ssrbool seq eqtype ssrnat.
-
+Set Implicit Arguments.
 
 
 Definition get_block (CFG:mcfg) fid bid :=
@@ -21,10 +21,93 @@ Definition get_block (CFG:mcfg) fid bid :=
   mret blk
 .
 
+Fixpoint wf_phis (phis:seq (local_id * phi)) (bk:block_id) (e:env) :=
+  match phis with
+  | nil => true
+  | (l, Phi typ l2) :: tl => match assoc AstLib.RawID.eq_dec bk l2 with
+                             | Some op => match eval_op e (Some typ) op with
+                                          | inr _ => wf_phis tl bk e
+                                          | inl _ => false
+                                          end
+                                            
+                             | None => false                        
+                          end
+                            
+  end.
 
-Definition block_uid b :=  ( NoDup ((map fst (blk_code b)) ++ ( blk_term_id b ) :: nil)).
+
+
+Definition branch_correct (m:mcfg) := forall p e br phis n_pc,
+    fetch m p = Some (Term (TERM_Br_1 br)) -> find_block_entry m (fn p) br = Some (BlockEntry phis n_pc) ->
+    wf_phis phis (bk p) e.
+
+
+
+Definition block_uid m := forall fn bk b, get_block m fn bk = Some b -> ( NoDup ((map fst (blk_code b)) ++ ( blk_term_id b ) :: nil)).
+
+
+Fixpoint compare_length A B (l1: seq A) (l2: seq B) : Prop :=
+  match l1, l2 with
+  | nil, nil => True
+  | _ :: tl, _ :: tl1 => compare_length tl tl1
+  | _, _ => False
+  end.
+
+
+
+Lemma compare_length_trans : forall A B C (l1: seq A) (l2: seq B) (l3: seq C),
+    compare_length l1 l2 -> compare_length l2 l3 -> compare_length l1 l3.
+Proof. induction l1, l2, l3; simpl in *; eauto. intros. inversion H. Qed.
+
+
+Lemma compare_length_sym : forall A B (l1: seq A) (l2: seq B), compare_length l1 l2 = compare_length l2 l1.
+  Proof. induction l1, l2; simpl in *; eauto. Qed. 
+
+Lemma map_preserves_length : forall A B C (l1:seq A) (l2:seq B) (f:B -> C) (l3:seq C), compare_length l1 l2 ->
+                                                                                       map f l2 = l3 -> compare_length l1 l3.
+Proof. induction l1, l2, l3; simpl in *; eauto; intros.
+       +induction l3. simpl in *. inversion H0. simpl in *. inversion H0. simpl in *. inversion H. simpl in *. inversion H0. simpl in *. inversion H0. subst. inversion H0. eapply IHl1 in H; eauto. Qed.
+
+Lemma map_monad_partition : forall  t val l2 l3 e, 
+    map_monad (fun '(t, op) => eval_op e (Some t) op) ((t, val)::l2) = inr l3 ->
+    exists res1 res2,  eval_op e (Some t) val = inr res1 /\ map_monad  (fun '(t, op) => eval_op e (Some t) op) l2 = inr res2 /\ l3 = res1 :: res2.
+Proof. intros. simpl in *. destruct (eval_op e (Some t) val). inversion H. 
+destruct ( map_monad (fun '(t, op) => eval_op e (Some t) op) l2). inversion H. inversion H. eauto. Qed.
+
+
+Lemma map_moad_preserves_length : forall l2 l3 e,  map_monad (fun '(t, op) => eval_op e (Some t) op) l2 = inr l3 -> compare_length l2 l3.
+Proof. induction l2. intros. simpl in *. destruct l3. eauto. inversion H.
+
+
+
+       destruct a.
+
+       intros. dupl H.  eapply map_monad_partition in H0.
+
+       destruct H0. destruct H0. destruct H0. destruct H1. rewrite H2.
+       simpl. eapply IHl2. eauto. Qed.
+
+
+(*WF call instructions - Call instructions are wff if they have the same number of arguments as the prototype of the instruction being called*)
 
 
 
 
-Definition wf_program (m:mcfg) := forall fn bk b, get_block m fn bk = Some b -> block_uid b.
+(*                 compare_length (df_args d0) args0 ->
+                 compare_length args0 l ->
+                  compare_length args l0 -> 
+
+                 combine (df_args d0) l = combine (df_args d0) l0 -> l = l0
+
+ *)
+
+
+
+
+
+Definition wf_call_instr (m:mcfg) := forall p fn func args t,
+  fetch m p = Some (CFG.Step (INSTR_Call t args)) -> snd t = ID_Global fn ->
+  find_function m fn = Some func -> compare_length (df_args func) args.
+
+Inductive wf_program (m:mcfg) : Prop :=
+  | wf_program_intro : forall (wf_call: wf_call_instr m)(buid: block_uid m) (bcor: branch_correct m), wf_program m.
