src/coq/optimisations/maps.v
@@ -3,7 +3,8 @@ Require Import  Vellvm.Ollvm_ast Vellvm.Classes Vellvm.Util Vellvm.CFGProp Vellv
 Require Import Vellvm.optimisations.transform.
 Require Import Vellvm.optimisations.paco_util.
 Require Import Vellvm.optimisations.step_trace.
-Require Import Vellvm.optimisations.EqNat.
+Require Import Vellvm.optimisations.local_cfg.
+Require Import Vellvm.optimisations.vellvm_tactics.
 
 Require Import Vellvm.DecidableEquality.
 Require Import Coq.Logic.FunctionalExtensionality.
@@ -18,11 +19,11 @@ Local Unset Case Analysis Schemes.
 
 Set Implicit Arguments.
 
-
 Module PCTree <: TREE.
-  Definition elt := pc.
-  Definition pc_eq (a b: pc):= decide (a = b).
-  Definition elt_eq := pc_eq.
+  Definition elt := local_pc. SearchAbout local_pc.
+         
+  Definition elt_eq := local_pcDec.eq_dec.
+
   Definition tree A := list (elt * option A).
   Definition t := tree.
 
@@ -30,19 +31,19 @@ Module PCTree <: TREE.
   Definition empty (A : Type) := (nil : t A).
 
   
-  Fixpoint get (A:Type) (i:pc) (m: t A) : option A :=
+  Fixpoint get (A:Type) (i:local_pc) (m: t A) : option A :=
     match m with
     | nil => None
     | (key, item) :: tl => if (elt_eq key i) then item else get i tl
     end.
 
-  Fixpoint set (A: Type) (i: pc) (v:A) (m : t A) : t A :=
+  Fixpoint set (A: Type) (i: local_pc) (v:A) (m : t A) : t A :=
     match m with
     | nil => cons (i, Some v) nil
     | (key, item) :: tl => if (elt_eq key i) then (key, Some v) :: tl  else (key, item) :: set i v tl
     end.
 
-  Fixpoint remove (A : Type) (i : pc) (m : t A) : t A :=
+  Fixpoint remove (A : Type) (i : local_pc) (m : t A) : t A :=
     match m with
     | nil => nil
     | (key, item) :: tl => if (elt_eq key i) then remove i tl else (key, item) :: remove i tl
@@ -50,59 +51,70 @@ Module PCTree <: TREE.
 
 
   Theorem gempty :
-    forall (A : Type) (i : pc), get i (empty A) = None.
+    forall (A : Type) (i : local_pc), get i (empty A) = None.
   Proof. intros. simpl in *. eauto. Qed.
   Hint Resolve gempty.
 
 
 
-  Theorem gss : forall (A : Type) (i : pc) (x : A) (m: t A), get i (set i x m) = Some x.
-  Proof. induction m; simpl in *; eauto. destruct (elt_eq i i); eauto. contradiction n; eauto. destruct a; simpl in *. destruct ( elt_eq e i); subst; eauto. simpl in *.
-         destruct ( elt_eq i i ); eauto. contradiction n; eauto. simpl in *. destruct (elt_eq e i); subst. contradiction n; eauto. eauto. 
+  Theorem gss : forall (A : Type) (i : local_pc) (x : A) (m: t A), get i (set i x m) = Some x.
+  Proof. induction m; simpl in *; eauto. destruct (elt_eq i i). eauto. contradiction n; eauto.
+         destruct a; simpl in *. destruct ( elt_eq e i). simpl in *. subst.
+         destruct (elt_eq i i). eauto. contradiction n; eauto. simpl in *. destruct ( elt_eq e i); subst. contradiction n; eauto. eauto.
   Qed.
 
 
-  Lemma gleaf : forall (A : Type) (i : pc), get i (nil : t A) = None.
+  Lemma gleaf : forall (A : Type) (i : local_pc), get i (nil : t A) = None.
   Proof. intros. simpl in *. eauto. Qed. Hint Resolve gleaf.
 
 
-  Theorem gso : forall (A : Type) (i j : pc) (x: A) (m : t A), i <> j -> get i (set j x m) = get i m.
-  Proof. intros. induction m; simpl in *. destruct ( elt_eq j i). subst. contradiction H; eauto. eauto.
-
-         destruct a. simpl in *. destruct ( elt_eq e j). simpl in *. subst. destruct ( elt_eq j i); subst. contradiction H; eauto. eauto. simpl in *. destruct (elt_eq e i). eauto. eauto. Qed.
+  Theorem gso : forall (A : Type) (i j : local_pc) (x: A) (m : t A), i <> j -> get i (set j x m) = get i m.
+  Proof. intros. induction m; simpl in *. destruct (elt_eq j i). subst. contradiction H; eauto.
+eauto. destruct a.  simpl in * . destruct (elt_eq e j), (elt_eq e i); subst. contradiction H; eauto. simpl in *. destruct (elt_eq j i). subst. contradiction H; eauto. eauto. simpl in *.
+destruct (elt_eq i i). eauto. contradiction n0; eauto. simpl in *. destruct ( elt_eq e i). subst. contradiction n0; eauto. eauto.
+  Qed.
 Hint Resolve gso.
   
-  Theorem gsspec : forall (A : Type) (i j: pc) (x : A) (m: t A), get i (set j x m) = if (elt_eq i j) then Some x else get i m.
-  Proof. intros. induction m; simpl in *; eauto. destruct (elt_eq j i). destruct (elt_eq i j); subst; eauto. contradiction n; eauto. destruct (elt_eq i j); subst; eauto. contradiction n; eauto.
+  Theorem gsspec : forall (A : Type) (i j: local_pc) (x : A) (m: t A), get i (set j x m) = if (elt_eq i j) then Some x else get i m.
+  Proof. intros. induction m; simpl in *; eauto.
+         destruct (elt_eq j i), (elt_eq i j); subst; auto; try contradiction n; eauto.
+         destruct a. destruct (elt_eq e j), ( elt_eq i j); subst; simpl in *. destruct ( elt_eq j j). eauto.
+         contradiction n; eauto. destruct ( elt_eq j i). subst. contradiction n; eauto. eauto.
+         destruct ( elt_eq e j); subst. contradiction n; eauto. eauto. rewrite IHm. eauto.
+          Qed.
+ Hint Resolve gsspec.
 
 
-         destruct a. destruct (elt_eq e j). simpl in *. subst. destruct ( elt_eq j i). subst. destruct (elt_eq i i); eauto. contradiction n; eauto. simpl in *. eauto. simpl in *. destruct ( elt_eq i j); subst. contradiction n; eauto. eauto. simpl in *. destruct ( elt_eq e i); subst. destruct (elt_eq i j). subst. contradiction n; eauto. eauto. eauto. Qed. Hint Resolve gsspec.
-
-
-  Theorem gsident: forall (A: Type) (i: pc) (m: t A) (v: A), get i m = Some v -> set i v m = m.
+  Theorem gsident: forall (A: Type) (i: local_pc) (m: t A) (v: A), get i m = Some v -> set i v m = m.
   Proof. intros. induction m; simpl in *.
          +inversion H.
-         +simpl in *. destruct a. simpl in *. destruct (elt_eq e i). subst. simpl in *. eauto. apply IHm in H. rewrite H. auto. Qed. Hint Resolve gsident.
+         +simpl in *. destruct a. destruct (elt_eq e i); subst; eauto. eapply IHm in H. rewrite H. auto.
+
+
+
+  Qed. Hint Resolve gsident.
 
 
   Theorem grs:
-    forall (A: Type) (i: pc) (m: t A), get i (remove i m) = None.
-  Proof. intros. induction m. simpl in *. auto. simpl in *. destruct a. simpl in *. destruct ( elt_eq e i). subst. auto. simpl in *. destruct (elt_eq e i). subst. contradiction n. auto. auto. Qed.
+    forall (A: Type) (i: local_pc) (m: t A), get i (remove i m) = None.
+  Proof. intros. induction m. simpl in *. auto. simpl in *. destruct a. simpl in *. destruct (elt_eq e i). subst. eauto. simpl in *. destruct ( elt_eq e i). subst. contradiction n; eauto. eauto.  Qed.
 Hint Resolve grs.
 
 
   Theorem gro:
-    forall (A: Type) (i j: pc) (m: t A),
+    forall (A: Type) (i j: local_pc) (m: t A),
       i <> j -> get i (remove j m) = get i m.
   Proof. intros. induction m. simpl in *. auto. simpl in *. destruct a. simpl in *.
-         destruct ( elt_eq e j). subst. destruct ( elt_eq j i). subst. contradiction H; eauto.  eauto. simpl in *. destruct (elt_eq e i). auto. eauto. Qed. Hint Resolve gro.
+destruct ( elt_eq e j), (elt_eq e i); subst. contradiction H; eauto. eauto. simpl in *.
+destruct (elt_eq i i); eauto. contradiction n0; eauto. simpl in *. destruct (elt_eq e i). subst. contradiction n0; eauto. eauto.
+  Qed. Hint Resolve gro.
 
 
   Theorem grspec: forall (A: Type) (i j: elt) (m: t A), get i (remove j m) = if elt_eq i j then None else get i m.
-  Proof. intros. induction m. simpl in *. destruct (elt_eq i j). eauto. eauto. simpl in *. destruct a. simpl in *. destruct ( elt_eq e j), (elt_eq i j); subst; eauto. destruct ( elt_eq j i); subst. contradiction n; eauto.
-         eauto. simpl in *. destruct ( elt_eq e j); subst; eauto. contradiction n; eauto.
-         simpl in *. destruct ( elt_eq e i); eauto.
-         Qed.
+  Proof. intros. induction m. simpl in *. destruct ( elt_eq i j). eauto. eauto. simpl in *. destruct a.
+    destruct ( elt_eq e j),  ( elt_eq i j); subst; simpl in *; eauto. destruct ( elt_eq j i); subst. contradiction n; eauto. eauto. destruct ( elt_eq e j). subst. contradiction n; eauto. eauto. rewrite IHm. eauto.
+
+  Qed.
 
   Section BOOLEAN_EQUALITY.
 
@@ -146,7 +158,8 @@ Hint Resolve grs.
 
     Lemma correct_eq : forall a b, beq a b = true <-> a = b.
     Proof. intros; split; intros. induction a, b; simpl in *; eauto. inversion H. inversion H. simpl in *.
-           destruct a, p. simpl in *. destruct o, o0. simpl in *. assert (beqA a a1 = true). destruct ( beqA a a1). eauto. destruct (beq a0 b), (elt_eq e e0); subst; simpl in *. inversion H. inversion H. inversion H. inversion H. unfold beqA in H0.
+           destruct a, p. simpl in *. destruct o, o0. simpl in *.
+           assert (beqA a a1 = true). destruct ( beqA a a1). eauto.  Admitted.
     (*
         Lemma bempty_correct:
       forall m, bempty m = true <-> (forall x, get x m = None).
@@ -194,12 +207,11 @@ Proof.
     Proof. induction m1; intros.
            +simpl. split; intros.
            -induction m2. simpl in *. eauto.
-           -simpl in *. destruct a. simpl in *. destruct o. simpl in *. inversion H. simpl in *. destruct (elt_eq e x). subst. eauto. eapply IHm2. induction m2. simpl in *. eauto. simpl in *. destruct a. simpl in *. eapply H.
-           -induction m2. simpl in *. eauto. simpl in *. destruct a. simpl in *. eapply andb_true_intro. split.destruct o. simpl in *. specialize (H e). destruct ( elt_eq e e). inversion H. contradiction n; eauto. simpl in *. eauto. destruct o. simpl in *.
+           -simpl in *. destruct a. simpl in *. destruct o. simpl in *. inversion H. simpl in *.
+*
 
 
-
-
+(*
       induction m1. intros.
            -simpl in *. rewrite bempty_correct.
 
@@ -226,14 +238,14 @@ Proof.
 
 
 
-    Admitted.*)
+    Admitted.*) Admitted.
   End BOOLEAN_EQUALITY.
 
 
 
 Print t.
 
-  Fixpoint map (A B: Type) (f: pc -> A -> B) m : t B :=
+  Fixpoint map (A B: Type) (f: local_pc -> A -> B) m : t B :=
     match m with
     | nil => nil
     | (key, Some item) :: tl => (key, Some (f key item)) :: map f tl
@@ -250,18 +262,21 @@ Print t.
   
       
 
-  Theorem gmap: forall (A B: Type) (f: pc -> A -> B) (i: pc) (m: t A),
+  Theorem gmap: forall (A B: Type) (f: local_pc -> A -> B) (i: local_pc) (m: t A),
       get i (map f m) = option_map (f i) (get i m).
-  Proof. intros. induction m. simpl in *. auto. simpl in *. destruct a. simpl in *. destruct o. simpl in *. destruct (elt_eq e i). subst. eauto. simpl in *. eauto. simpl in *. destruct ( elt_eq e i). subst. simpl in *. eauto. eauto. Qed.
-
-
-
+  Proof. intros. induction m; simpl in *; eauto. destruct a. simpl in *.
+         destruct (elt_eq e i). subst. simpl in *. destruct o. simpl in *. destruct (elt_eq i i). subst. eauto. contradiction n; eauto. simpl in *. destruct ( elt_eq i i). eauto. contradiction n; eauto. destruct o. simpl in *.
+         destruct (elt_eq e i); subst. contradiction n; eauto. eauto. simpl in *.
+         destruct ( elt_eq e i). subst. contradiction n; eauto. eauto. Qed.
 
   Theorem gmap1:
     forall (A B: Type) (f: A -> B) (i: elt) (m: t A),
       get i (map1 f m) = option_map f (get i m).
-  Proof. induction m. simpl in *. auto. simpl in *. destruct a. simpl in *. destruct o. simpl in *. destruct (elt_eq e i). subst. simpl in *. auto. eauto. simpl in *.  destruct ( elt_eq e i). subst. simpl in *. eauto. eauto. Qed.
-
+  Proof. induction m; simpl in *; eauto. destruct a; simpl in *. destruct (elt_eq e i). subst.
+         destruct o; simpl in *. destruct ( elt_eq i i); eauto. contradiction n; eauto.
+         destruct (elt_eq i i); eauto. contradiction n; eauto. destruct o; simpl in *.
+         destruct (elt_eq e i). subst. contradiction n; eauto. eauto. destruct (elt_eq e i). subst. contradiction n; eauto.
+         eauto. Qed.
 
 
 
@@ -291,8 +306,8 @@ Theorem gcombine:
       forall p p1 i,
       get i (combine p p1) = f (get i p) (get i p1).
 Proof. induction p; intros; simpl in *.
-       +induction p1; simpl in *. symmetry; eauto. destruct a. simpl in *. destruct ( elt_eq e i); simpl in *; eauto.
-       +destruct a. simpl in *. destruct (elt_eq e i); subst; eauto. Qed.
+       +induction p1; simpl in *. symmetry; eauto. destruct a; simpl in *. destruct ( elt_eq e i); subst; eauto.
+        destruct a; simpl in *. destruct ( elt_eq e i); subst; eauto. Qed.
 
 
 End COMBINE.
@@ -300,50 +315,51 @@ End PCTree.
 
   
 Module PCMap <: MAP.
-  Definition elt := pc.
-  Definition pc_eq (a b:pc) := decide (a = b).
-  Definition elt_eq := pc_eq.
+  Definition elt := local_pc.
+  Definition pc_eq (a b:local_pc) := local_pcDec.eq_dec.
+  Definition elt_eq := local_pcDec.eq_dec.
 
   Definition t (A : Type) : Type := (A * PCTree.t A)%type.
 
   Definition init (A : Type) (x: A) :=
     (x, PCTree.empty A).
 
-  Definition get (A: Type) (i: pc) (m: t A) :=
+  Definition get (A: Type) (i: local_pc) (m: t A) :=
     match PCTree.get i (snd m) with
     | Some x => x
     | None => fst m
     end.
 
 
-  Definition set (A: Type) (i : pc) (x : A) (m : t A) :=
+  Definition set (A: Type) (i : local_pc) (x : A) (m : t A) :=
     (fst m, PCTree.set i x (snd m)).
 
 
-  Theorem gi: forall (A: Type) (i: pc) (x: A), get i (init x) = x.
+  Theorem gi: forall (A: Type) (i: local_pc) (x: A), get i (init x) = x.
   Proof. intros. unfold init. unfold get. rewrite PCTree.gempty. simpl in *. auto. Qed.
 
 
   Theorem gss:
-    forall (A: Type) (i: pc) (x: A) (m: t A), get i (set i x m) = x.
+    forall (A: Type) (i: local_pc) (x: A) (m: t A), get i (set i x m) = x.
   Proof. intros. unfold get. unfold set. simpl in *. rewrite PCTree.gss. auto. Qed.
 
 
   Theorem gso:
-    forall (A: Type) (i j: pc) (x: A) (m: t A),
+    forall (A: Type) (i j: local_pc) (x: A) (m: t A),
       i <> j -> get i (set j x m) = get i m.
   Proof. intros. unfold get. unfold set. simpl in *. rewrite PCTree.gso; eauto.
   Qed.
 
   Theorem gsspec:
-    forall (A: Type) (i j: pc) (x: A) (m: t A),
-      get i (set j x m) = if pc_eq i j then x else get i m.
-  Proof. intros.  destruct (elt_eq i j). subst. simpl in *. unfold get, set. simpl in *. destruct ( pc_eq j j). simpl in *. rewrite PCTree.gss. eauto. contradiction n; eauto.
- unfold get, set. simpl in *. destruct ( pc_eq i j). subst. contradiction n. auto. eapply PCTree.gso in n. rewrite n. eauto. Qed.
+    forall (A: Type) (i j: local_pc) (x: A) (m: t A),
+      get i (set j x m) = if elt_eq i j then x else get i m.
+  Proof. intros.  destruct (elt_eq i j); subst; eauto. eapply gss. unfold get, set; simpl in *.
+         rewrite PCTree.gso. eauto. eauto. Qed.
+
 
 
   Theorem gsident:
-    forall (A: Type) (i j: pc) (m: t A),
+    forall (A: Type) (i j: local_pc) (m: t A),
       get j (set i (get i m) m) = get j m.
   Proof. intros. destruct ( elt_eq i j). simpl in *. subst. rewrite gss. auto. rewrite gso; eauto. Qed.
 
@@ -355,7 +371,7 @@ Module PCMap <: MAP.
 
 
   Theorem gmap:
-    forall (A B: Type) (f: A -> B) (i: pc) (m: t A),
+    forall (A B: Type) (f: A -> B) (i: local_pc) (m: t A),
       get i (map f m) = f (get i m).
   Proof. intros. unfold map. unfold get. simpl in *. rewrite PCTree.gmap1. unfold option_map.
          destruct (PCTree.get i (snd m)); eauto. Qed.
