src/coq/optimisations/Kildall/backwards_kildall.v
@@ -1,0 +1,142 @@
+Require Import Vellvm.CFG.
+Require Import Vellvm.Ollvm_ast.
+Require Import Coq.Lists.List.
+Require Import Coq.Arith.EqNat.
+Require Import Vellvm.optimisations.Kildall.kildall.
+Require Import Vellvm.optimisations.Kildall.lattice.
+Require Import Vellvm.optimisations.maps.
+Set Implicit Arguments.
+
+
+
+(*
+
+Module Type BACKWARD_DATAFLOW_SOLVER.
+
+  Declare Module L: SEMILATTICE.
+
+    Variable code: mcfg. (*MCFG*)
+    Variable fetch : mcfg -> pc -> option cmd. (*MCFG -> PC -> INSTR*)
+
+  
+  Parameter fixpoint:
+    forall (code: mcfg) (successors: pc -> list pc)
+           (transf: pc -> L.t -> L.t),
+    option (PCMap.t L.t).
+
+    Axiom fixpoint_solution:
+    forall (code: mcfg) successors transf res n instr s,
+    fixpoint code successors transf = Some res ->
+    fetch code n = Some instr -> In s (successors n) ->
+    (forall n a, fetch code n = None -> L.eq (transf n a) L.bot) ->
+    L.ge res!!n (transf s res!!s).
+
+
+      Parameter fixpoint_allnodes:
+    forall (code: mcfg) (successors: pc -> list pc)
+           (transf: pc -> L.t -> L.t),
+    option (PCMap.t L.t).
+
+      
+  Axiom fixpoint_allnodes_solution:
+    forall (code: mcfg) successors transf res n instr s,
+    fixpoint_allnodes code successors transf = Some res ->
+    fetch code n = Some instr -> In s (successors n) ->
+    L.ge res!!n (transf s res!!s).
+
+End BACKWARD_DATAFLOW_SOLVER.
+
+
+Module Backward_Dataflow_Solver (LAT: SEMILATTICE) (NS: NODE_SET):
+                   BACKWARD_DATAFLOW_SOLVER with Module L := LAT.
+
+
+  Definition fixpoint_from (start: state) : option (PCMap.t L.t) :=
+  PrimIter.iterate _ _ step start.
+
+
+
+Definition fixpoint_nodeset (enodes: NS.t) :=
+  fixpoint_from (start_state_nodeset enodes).
+
+
+Definition fixpoint :=
+  DS.fixpoint_nodeset
+    (make_predecessors code successors) (fun l => l)
+    transf exit_points.
+
+(*Lemma make_predecessors_correct_1:
+  forall n instr s,
+  code!n = Some instr -> In s (successors instr) ->
+  In n make_predecessors!!!s.
+Proof.
+  intros until s.
+  set (P := fun m p => m!n = Some instr -> In s (successors instr) ->
+                       In n p!!!s).
+  unfold make_predecessors.
+  apply PTree_Properties.fold_rec with (P := P); unfold P; intros.
+ extensionality   apply H0; auto. rewrite H; auto.
+ base case   rewrite PTree.gempty in H; congruence.
+ inductive case  apply add_successors_correct.
+  rewrite PTree.gsspec in H2. destruct (peq n k).
+  inv H2. auto.
+  auto.
+Qed.
+
+Lemma make_predecessors_correct_2:
+  forall n instr s,
+  code!n = Some instr -> In s (successors instr) ->
+  exists l, make_predecessors!s = Some l /\ In n l.
+Proof.
+  intros. exploit make_predecessors_correct_1; eauto.
+  unfold successors_list. destruct (make_predecessors!s); simpl; intros.
+  exists l; auto.
+  contradiction.
+Qed.
+*)
+
+(*Definition fixpoint_allnodes :=
+  DS.fixpoint_allnodes
+    (make_predecessors code successors) (fun l => l)
+    transf.
+
+Theorem fixpoint_allnodes_solution:
+  forall res n instr s,
+  fixpoint_allnodes = Some res ->
+  code!n = Some instr -> In s (successors instr) ->
+  L.ge res!!n (transf s res!!s).
+Proof.
+  intros.
+  exploit (make_predecessors_correct_2 code); eauto. intros [l [P Q]].
+  unfold fixpoint_allnodes in H.
+  eapply DS.fixpoint_allnodes_solution; eauto.
+Qed.
+ *)*)
+
+
+
+Fixpoint foldr A B (f:A -> B -> B) (l:list A) (c: B) :=
+  match l with
+  | nil => c
+  | hd :: tl => f hd (foldr  f tl c)
+  end.
+
+
+Lemma equiv : forall (f:nat -> nat -> nat) (a:nat) (xs:nat) (ys:list nat), f xs (foldr f ys a) = foldr f (xs::ys) a.
+Proof. induction ys. simpl in *. eauto. simpl in *. eauto. Qed.
+
+
+
+
+
+
+Definition func (a:nat) (l: nat) : nat :=
+  if beq_nat a 0 then a + l else l.
+
+
+
+Lemma equiv1 : forall l c, foldr func l c = c.
+Proof. induction l. simpl in *. eauto. simpl in *. unfold func. simpl in *. destruct (PeanoNat.Nat.eqb a 0) eqn:?. symmetry in Heqb. eapply beq_nat_eq in Heqb. subst. simpl. eauto. eauto. Qed.
+
+
+Print incr_pc. 
