src/coq/optimisations/Kildall/congruence_proof_kildall.v
@@ -6,13 +6,13 @@ Require Import Vellvm.optimisations.Kildall.congruence_definition_kildall.
 Require Import Vellvm.optimisations.Kildall.valueanalysis.
 Require Import Vellvm.optimisations.Kildall.valuedomain.
 Require Import Vellvm.optimisations.Kildall.static_eval.
+Require Import Vellvm.optimisations.vellvm_tactics.
+Require Import Vellvm.optimisations.local_cfg.
 
 Require Import Vellvm.optimisations.maps.
 
-Print sound_state.
 
 Require Import Vellvm.optimisations.SSA_semantics.
-Require Import Vellvm.optimisations.vellvm_tactics.
 
 Require Import Vellvm.DecidableEquality.
 Require Import Coq.Logic.FunctionalExtensionality.
@@ -22,6 +22,49 @@ Require Import Vellvm.Effects.
 From mathcomp.ssreflect
 Require Import ssreflect ssrbool seq eqtype ssrnat.
 Print sound_stack.
+
+
+Lemma find_function_entry_unaffected_V1: forall m o,
+    find_function_entry (modul_opt o m) = find_function_entry m.
+Proof. intros. apply functional_extensionality.
+       intros. rewrite find_function_entry_unaffected; auto. Qed.
+
+
+Lemma jump_unaffected_v1 : forall o m, jump (modul_opt o m) = jump m.
+Proof. intros. apply functional_extensionality. intros.
+       apply functional_extensionality. intros.
+       apply functional_extensionality. intros.
+       apply functional_extensionality. intros.
+       apply functional_extensionality. intros.
+       apply jump_unaffected. Qed.
+
+
+Lemma stack_false_l : forall t (s:stack),  t :: s = s -> False.
+Proof. intros. induction s. simpl in *.
+       inversion H. apply IHs. inversion H.
+       subst. rewrite H2. eauto. Qed.
+
+Lemma stack_false_r : forall  t (s:stack),  s = t :: s -> False.
+Proof. intros. induction s. simpl in *.
+       inversion H. apply IHs. inversion H.
+       subst. rewrite <- H2. eauto. Qed.
+
+Lemma mem_false_r : forall (mem:seq dvalue) undef, mem = (mem ++ [:: undef])%list -> False.
+Proof. intros. induction mem. simpl in *.
+       inversion H. simpl in *. apply IHmem.
+       inversion H. subst. rewrite <- H1. auto. Qed.
+
+Lemma mem_false_l : forall (mem:seq dvalue) undef,  (mem ++ [:: undef])%list = mem -> False.
+Proof. intros. induction mem. simpl in *.
+       inversion H. apply IHmem. simpl in *.
+       inversion H. subst. rewrite H1. auto. Qed.
+
+
+
+Ltac break_congruence :=  break_inner_match_goal; simpl in *; eauto; try eapply trace_equiv_err; try eapply trace_equiv_fin.
+Ltac try_break_congruence := try (repeat break_congruence); simpl in *; eauto; try eapply trace_equiv_err; try eapply trace_equiv_fin.
+
+
 
 
 
@@ -44,109 +87,41 @@ Ltac break_goal := unfold find_function_entry in *; break_inner_match_goal; simp
 Ltac try_resolve := try (repeat break_goal); try constructor.
 
 
-Lemma find_function_entry_unaffected_V1: forall m o,
-                                                                                                  find_function_entry (modul_opt o m) = find_function_entry m. Proof. intros. apply functional_extensionality. intros. rewrite find_function_entry_unaffected; auto. Qed.
-
-
-Lemma jump_unaffected_v1 : forall o m, jump (modul_opt o m) = jump m.
-Proof. intros. apply functional_extensionality. intros.  apply functional_extensionality.
-       intros.  apply functional_extensionality. intros.  apply functional_extensionality. intros.  apply functional_extensionality. intros.  apply jump_unaffected. Qed.
-Print correct_instr1.
-
-
-Lemma stack_false_l : forall t (s:stack),  t :: s = s -> False.
-Proof. intros. induction s. simpl in *. inversion H. apply IHs. inversion H. subst. rewrite H2. eauto. Qed.
-
-Lemma stack_false_r : forall  t (s:stack),  s = t :: s -> False.
-Proof. intros. induction s. simpl in *. inversion H. apply IHs. inversion H. subst. rewrite <- H2. eauto. Qed.
-
-Print memory.
-Lemma mem_false_r : forall (mem:seq dvalue) undef, mem = (mem ++ [:: undef])%list -> False.
-Proof. intros. induction mem. simpl in *. inversion H. simpl in *. apply IHmem. inversion H. subst. rewrite <- H1. auto. Qed.
-
-Lemma mem_false_l : forall (mem:seq dvalue) undef,  (mem ++ [:: undef])%list = mem -> False.
-Proof. intros. induction mem. simpl in *. inversion H. apply IHmem. simpl in *. inversion H. subst. rewrite H1. auto. Qed.
-
-
-
-
-Ltac inv t := inversion t; subst; clear t; eauto.
-Ltac destr_eq t := destruct t eqn:?; simpl; eauto.
-Ltac destr t := destruct t; simpl; eauto.
-Ltac appl t y := generalize y; intro; apply t in y.
-
-Print Expr. Print typ. Print Ollvm_ast.typ.  Print instr.
-   
-                                                                                                                                                                           
 Lemma congruence_correct1 : forall o m st mem (correct_instr: correct_instr1 o m) (wf_program: wf_program m) (sstate: sound_state m st), trace_equiv (memD mem (sem m st)) (memD mem (sem (modul_opt o m) st)).
 Proof. 
   pcofix CIH. intros. pfold.
-  assert (memD mem (sem m st) = unroll(memD mem (sem m st))). destruct (memD mem (sem m st)); eauto. rewrite H. clear H.
+  assert (memD mem (sem m st) = unroll(memD mem (sem m st))).
+  destruct (memD mem (sem m st)); eauto. rewrite H. clear H.
   assert ( (memD mem (sem (modul_opt o m) st)) = unroll  (memD mem (sem (modul_opt o m) st))).
-
-
-
   destruct  (memD mem (sem (modul_opt o m) st)); eauto. rewrite H. clear H.
 
-
-
   dupl correct_instr.
-
-
-
-  
-simpl in *. unfold stepD. destruct st. destruct p. destruct p. 
-
-rewrite fetch_helper_equiv. rewrite <- incr_pc_unaffected.
-unfold fetch_helper.
-
-unfold correct_instr1 in *.
-unfold fetch, incr_pc in *.
-simpl in *.
+  simpl in *. unfold stepD. destruct st. destruct p. destruct p.
+  rewrite fetch_helper_equiv. rewrite <- incr_pc_unaffected.
+  unfold fetch_helper. unfold correct_instr1 in *. unfold fetch, incr_pc in *.
+  simpl in *.
 
 
 destr_eq (find_function m fn).
 destr_eq ( find_block (blks (df_instrs d)) bk).
-destr_eq (block_to_cmd b pt ).
-destr p.
-destr c.
-destr o0.
+destr_eq (block_to_cmd b pt).
+
+destruct p. destruct c. destruct o0; simpl in *; eauto.
 specialize (correct_instr mem fn bk pt i e s i0).
+subst. destruct pt.
+
 
 appl correct_instr wf_program.
 unfold exec_code1 in wf_program. simpl in *. 
 
 rewrite  find_function_entry_unaffected_V1.
 inv sstate.
-unfold individual_step in *; simpl in *. destruct pt; simpl in *.
-destruct ( o {| fn := fn; bk := bk; pt := IId id |} m (IId id, i)), i; simpl in *; eauto; unfold  lift_err_d in *; try (repeat break_goal); try inv wf_program.
+unfold individual_step in *; simpl in *.
 
+destruct ( o {| fn := fn; bk := bk; pt := IId id |} m (IId id, i)), i; simpl in *; eauto; unfold  lift_err_d; repeat (break_goal); try inv wf_program; try constructor; try right; try eapply CIH; intros; eauto.
+destruct op0.
 
-
-
-
-
-  +assert (fetch m (mk_pc fn bk (IId id)) = Some (CFG.Step (INSTR_Op op0))). unfold fetch. simpl in *. rewrite Heqo0. rewrite Heqo1. rewrite Heqo2. eauto.
-
-  +assert (incr_pc  m (mk_pc fn bk (IId id)) = Some (mk_pc fn bk i0)). unfold incr_pc; simpl. rewrite Heqo0. rewrite Heqo1. rewrite Heqo2. eauto.
-
-
-   
-   constructor. right. eapply CIH; intros; eauto; destr_eq op; destr_eq op0.
-subst. eapply sound_succ_state. eapply AN. eapply H. unfold get_successors; simpl in *; rewrite H; rewrite H0; simpl in *; left; eauto. unfold transfer'; rewrite H.  eauto. 
-apply ematch_update; eauto. 
-
-destruct e1; simpl in *; eauto; try constructor; try inversion Heqe0; eauto; unfold eval_expr in *; unfold eval_aenv_expr; simpl in *; try destruct t; try destruct sz; try constructor; try destruct p; try constructor; try destruct p; try constructor. try destruct p; try constructor. try destruct p; try constructor. try destruct p; try constructor. try destruct p; try constructor. destruct p; try constructor. destruct v1; try constructor. destruct e1; try constructor. destruct v2; try constructor. destruct e1; try constructor.  simpl in *. inversion Heqe0. simpl. eauto. destruct v1; try constructor. destruct e1; try constructor. destruct v2; try constructor. destruct e1; try constructor; simpl in *; try inversion H2; try constructor. destruct v1; try constructor. destruct e1; try constructor. destruct v2; try constructor. destruct e1; try constructor; simpl in *. inversion H2; eauto. destruct p; try constructor.  destruct p; try constructor. destruct p; try constructor. destruct p; try constructor. destruct p; try constructor. destruct v1; try constructor. destruct e1; try constructor. destruct v2; try constructor. destruct e1; try constructor; simpl in *. inversion H2; eauto. destruct v1; try constructor. destruct e1; try constructor. destruct v2; try constructor. destruct e1; try constructor; simpl in *. inversion H2; eauto. destruct v1, v2; try constructor. destruct e1, e2; try constructor; simpl in *. inversion H2; eauto. eauto.
-
-
-
-
-
-
-
-
-
-
+eapply sound_succ_state; eauto; unfold successor_pc; unfold transfer'; unfold CFG.fetch; unfold fetch; unfold cfg_to_cmd; unfold pc_to_local_pc; simpl in *; try rewrite Heqo0; try rewrite Heqo1; try rewrite Heqo2; simpl in *; eauto; eapply ematch_update; eauto.
 
 
 
@@ -156,38 +131,61 @@ eapply mem_false_l in H; inversion H.
 
 
 
-
-
-
-constructor. right. eapply CIH; intros; eauto. eapply sound_succ_state; try eapply AN.
-unfold fetch; simpl in *; rewrite Heqo0; rewrite Heqo1; try rewrite Heqo2; eauto.
-unfold get_successors; simpl in *; rewrite Heqo0; rewrite Heqo1; rewrite Heqo2; simpl in *; eauto.
-unfold transfer'; simpl in *; rewrite Heqo0; rewrite Heqo1; rewrite Heqo2; eauto.
-eapply ematch_update; eauto; try constructor. eauto.
+eapply sound_succ_state. simpl in *. eauto. unfold CFG.fetch. simpl in *. rewrite Heqo0. rewrite Heqo1. rewrite Heqo2. eauto. unfold successor_pc. simpl in *. rewrite Heqo0. rewrite Heqo1. rewrite Heqo2. simpl in *. eauto. simpl in *.  
+eauto. unfold transfer'. simpl in *. unfold pc_to_local_pc. simpl in *. unfold fetch. unfold cfg_to_cmd. simpl in *. rewrite Heqo1. rewrite Heqo2. eauto. eapply ematch_update; eauto. constructor. eauto. 
 
 
 
 
 eapply stack_false_r in H6; inversion H6.
-constructor. right. eapply CIH; intros; eauto. eapply sound_succ_state. eapply AN. unfold fetch. rewrite Heqo0; simpl in *; rewrite Heqo1; rewrite Heqo2; eauto. unfold get_successors; simpl in *; rewrite Heqo0; rewrite Heqo1; rewrite Heqo2; unfold find_function_entry; simpl in *; rewrite Heqo5; simpl in ; rewrite Heqo6; simpl in *; inversion H4; inversion H3; subst; eauto. unfold transfer'; simpl in *; rewrite Heqo0; try rewrite Heqo1; try rewrite Heqo2; eauto. eauto. econstructor; simpl in *; eauto. rewrite Heqo0; rewrite Heqo1; rewrite Heqo2; eauto.
+
+
+inversion wf_program0. subst. unfold wf_call_instr in *.
+specialize (wf_call {| fn := fn; bk := bk; pt := (IId id) |}). unfold CFG.fetch in *. simpl in *. rewrite Heqo0 in wf_call. rewrite Heqo1 in wf_call. rewrite Heqo2 in wf_call.
+
+rewrite Heqo3 in Heqo5. inversion Heqo5. subst. clear Heqo5. rewrite Heqo4 in Heqo6. inversion Heqo6.  subst. clear Heqo6. clear H3. clear H4. specialize (wf_call id1). specialize (wf_call d1).
+specialize (wf_call args0). specialize ( wf_call  (t, ID_Global id1)). simpl in *.
+
+
+
+assert (Some (CFG.Step (INSTR_Call (t, ID_Global id1) args0)) =
+            Some (CFG.Step (INSTR_Call (t, ID_Global id1) args0))) by eauto. eapply wf_call in H; eauto. eapply analyse_entrypoint in Heqo3; eauto. destruct Heqo3.  destruct H0. 
+econstructor.
+simpl in *. econstructor.
+simpl in *. eapply AN. eauto. eauto. simpl in *. rewrite Heqo0. rewrite Heqo1. rewrite Heqo2. eauto. simpl in *. eauto. simpl in *. eauto. eapply map_moad_preserves_length in Heqe0.
+
+eapply compare_length_trans. apply H. eapply Heqe0.
+
+
 
 
 eapply stack_false_r in H7; inversion H7.
 eapply stack_false_r in H6; inversion H6.
-symmetry in H; eapply mem_false_l in H; inversion H.
-eapply stack_false_l in H7; inversion H7.
+eapply mem_false_r in H; inversion H; eauto.
+eapply mem_false_r in H; inversion H; eauto.
 
 
-constructor. right. eapply CIH; intros; eauto. eapply sound_succ_state. eapply AN. unfold fetch; simpl; rewrite Heqo0; rewrite Heqo1; rewrite Heqo2; eauto. unfold get_successors; simpl in *; rewrite Heqo0; rewrite Heqo1; rewrite Heqo2; simpl in *; eauto. unfold transfer'; unfold fetch; simpl; rewrite Heqo0; rewrite Heqo1; rewrite Heqo2; eauto. eapply ematch_add; eauto. eauto.
 
 
-symmetry in H; eapply mem_false_l in H; inversion H.
 
-destr_eq op.
+eapply sound_succ_state; simpl in *; eauto; unfold transfer', CFG.fetch, successor_pc, fetch, cfg_to_cmd; simpl in *; try rewrite Heqo0; try rewrite Heqo1; try rewrite Heqo2; simpl in *; eauto; eapply ematch_update; eauto; try constructor.
 
-constructor. right. eapply CIH; intros; eauto. eapply sound_succ_state. eapply AN. unfold fetch; simpl; rewrite Heqo0; rewrite Heqo1; rewrite Heqo2; eauto. unfold get_successors; simpl in *; rewrite Heqo0; rewrite Heqo1; rewrite Heqo2; simpl in *; eauto. unfold transfer'; unfold fetch; simpl in *; rewrite Heqo0; rewrite Heqo1; rewrite Heqo2; eauto. unfold add_env. simpl in *. unfold eval_aenv_expr; simpl in *; destr_eq e0; simpl in *; try destr_eq t1; try inv Heqe0;
 
-                                                                                                                                                                                                                                                                                                                                                                                             try destr_eq sz; try destr_eq p; try destr_eq p0; try destr_eq p1; try destr_eq p2; try destr_eq p3; try destr_eq p4; try destr_eq p5; try destr_eq v1; try destr_eq e0; try destr_eq v2; try destr_eq e1; try inv H0; try eapply ematch_update; eauto; constructor; eauto. eauto.
+
+
+
+
+eapply mem_false_r in H; inversion H; eauto.
+
+
+
+destruct op.
+
+
+
+eapply sound_succ_state; simpl in *; eauto; unfold transfer', CFG.fetch, successor_pc, fetch, cfg_to_cmd; simpl in *; try rewrite Heqo0; try rewrite Heqo1; try rewrite Heqo2; simpl in *; eauto; eapply ematch_update; eauto.
+
+
 
 
 
@@ -195,49 +193,46 @@ eapply stack_false_l in H6; inversion H6.
 eapply mem_false_l in H; inversion H; eauto.
 
 
-constructor; right; eapply CIH; intros; eauto.
-
-
-eapply sound_succ_state. eapply AN. unfold fetch; simpl in *; rewrite Heqo0; rewrite Heqo1; rewrite Heqo2; simpl in *; eauto. unfold get_successors; simpl in *; rewrite Heqo0; rewrite Heqo1; rewrite Heqo2; simpl in *; eauto.
-
-
-unfold transfer'; simpl in *; eauto; rewrite Heqo0; rewrite Heqo1; rewrite Heqo2; eauto. eapply ematch_add; eauto. eauto.
-
-
-
-destr_eq ( o {| fn := fn; bk := bk; pt := IVoid n |} m (IVoid n, i)); destr_eq i; simpl in *; eauto; unfold  lift_err_d in *; try (repeat break_goal); try inv wf_program; try eapply stack_false_r in H7; try inv H7; try eapply stack_false_l in H7; try inv H7; try constructor; try right; try eapply CIH; intros; eauto.
+eapply sound_succ_state; simpl in *; eauto; unfold transfer', CFG.fetch, successor_pc, fetch, cfg_to_cmd; simpl in *; try rewrite Heqo0; try rewrite Heqo1; try rewrite Heqo2; simpl in *; eauto; eapply ematch_update; eauto; try constructor.
+eauto.
 
 
 
 
+(***************** IVOID*)
 
-eapply sound_succ_state; try eapply AN; unfold fetch; unfold transfer'; unfold get_successors; simpl; try rewrite Heqo0; try rewrite Heqo1; try rewrite Heqo2; auto; unfold find_function_entry; simpl in *; try rewrite Heqo5; try rewrite Heqo6; simpl. rewrite H4. right. left. rewrite H3. eauto.
-
-
-
-
-
-econstructor; eauto. simpl in *. rewrite Heqo0. rewrite Heqo1. exists (TYPE_Void, ID_Global id0), args0, n. rewrite Heqo2. eauto.
+rewrite  find_function_entry_unaffected_V1.
+inv sstate.
+unfold individual_step in *; simpl in *.
 
 
+appl correct_instr wf_program; eauto. unfold exec_code1 in wf_program. unfold individual_step in wf_program. simpl in *.
 
 
-
-
-eapply stack_false_l in H0. inversion H0.
+destruct (o {| fn := fn; bk := bk; pt := IVoid n |} m (IVoid n, i)), i; simpl in *; eauto; unfold  lift_err_d; repeat (break_goal); try inv   wf_program; try constructor; try right; try eapply CIH; intros; eauto.
 
 
 
+rewrite Heqo3 in Heqo5. inversion Heqo5. subst. clear Heqo5. rewrite Heqo4 in Heqo6. inversion Heqo6. subst. clear Heqo6. clear H4. clear H3. 
 
 
 
+inversion wf_program0. subst. unfold wf_call_instr in *.
+specialize (wf_call {| fn := fn; bk := bk; pt := (IVoid n) |}). unfold CFG.fetch in *. simpl in *. rewrite Heqo0 in wf_call. rewrite Heqo1 in wf_call. rewrite Heqo2 in wf_call.
+specialize (wf_call id0). specialize (wf_call d1). specialize (wf_call args0). specialize (wf_call  (TYPE_Void, ID_Global id0)). simpl in *. 
+
+assert ( Some (CFG.Step (INSTR_Call (TYPE_Void, ID_Global id0) args0)) =
+         Some (CFG.Step (INSTR_Call (TYPE_Void, ID_Global id0) args0))) by eauto. eapply wf_call in H; eauto.
+eapply analyse_entrypoint in Heqo3; eauto.
+destruct Heqo3. destruct H0.
+
+econstructor; simpl in *; eauto. econstructor; eauto. simpl in *. rewrite Heqo0. rewrite Heqo1.
 
 
+exists (TYPE_Void, ID_Global id0). exists args0. exists n. rewrite Heqo2. eauto. 
+ eapply map_moad_preserves_length in Heqe0.
 
-eapply sound_succ_state; try eapply AN. unfold fetch; simpl in *. rewrite Heqo0. rewrite Heqo1. rewrite Heqo2. eauto. unfold get_successors; simpl in *. rewrite Heqo0; rewrite Heqo1; rewrite Heqo2; simpl; eauto. unfold transfer'. simpl in *. rewrite Heqo0; rewrite Heqo1; rewrite Heqo2. eauto.
-eauto. eauto.
-
-
+eapply compare_length_trans. apply H. eapply Heqe0.
 
 
 
@@ -254,45 +249,115 @@ eauto. eauto.
 
 
 
+eapply stack_false_r in H7; inversion H7.
+eapply stack_false_l in H7; inversion H7.
 
 
-auto.
+
+eapply sound_succ_state; simpl in *; eauto; unfold transfer', CFG.fetch, successor_pc, fetch, cfg_to_cmd; simpl in *; try rewrite Heqo0; try rewrite Heqo1; try rewrite Heqo2; simpl in *; eauto; eapply ematch_update; eauto; try constructor.
+
+
 
 
 
 
 rewrite jump_unaffected_v1.
+simpl in *.
+inv sstate.
+destruct t; simpl in *; eauto; unfold lift_err_d; repeat (break_goal); try inv wf_program; constructor; right; eapply CIH; intros; eauto.
 
-unfold jump. destruct t; unfold  lift_err_d in *; try (repeat break_goal); subst; try inv Heqt; constructor; right; eapply CIH; intros; eauto; inv sstate. simpl in EM; simpl in AN; simpl in sstack.
-
-inv sstack. simpl in *. destruct q. simpl in *. destruct H1. destruct H. destruct H. destr_eq (find_function m fn0). destr_eq ( find_block (blks (df_instrs d0)) bk0). destr_eq (block_to_cmd b0 (IId id)). destr_eq p. simpl in *. destr_eq c. inv H. destr_eq o1. inv  H0. eapply sound_succ_state. eapply AN0. unfold fetch; simpl. rewrite Heqo3. rewrite Heqo4. rewrite Heqo5. eauto. unfold get_successors; simpl in *; rewrite Heqo3; rewrite Heqo4; rewrite Heqo5. simpl in *. destruct x. simpl in *. destruct i. simpl in *. unfold find_function_entry; simpl. destr_eq (find_function m id0).
-destr_eq ( find_block (blks (df_instrs d1)) (init (df_instrs d1))). simpl in *. eauto. unfold transfer'; simpl in *. rewrite Heqo3. rewrite Heqo4. rewrite Heqo5. eauto. simpl in *. eauto. eauto.
-inversion H0. inversion H. inversion H. inversion H. inversion H.
-
-
-
-simpl in *. inv sstack. simpl in *. destr H1. destr H. destr H. destr H. destr H0. destr H1. destr p. simpl in *. destr_eq (find_function m fn0). destr_eq ( find_block (blks (df_instrs d0)) bk0). destr_eq (block_to_cmd b0 (IVoid x1)). destr p. destr o1. inv H1. inv H2. eapply sound_succ_state.
-eapply H. unfold fetch; simpl. rewrite Heqo3. rewrite Heqo4. rewrite Heqo5. eauto. unfold get_successors; simpl in *. rewrite Heqo3. rewrite Heqo4. rewrite Heqo5. unfold find_function_entry. destr x. destr i. destr_eq (find_function m id). destr_eq ( find_block (blks (df_instrs d1)) (init (df_instrs d1))). unfold transfer'; simpl. rewrite Heqo3. rewrite Heqo4. rewrite Heqo5. simpl in *. eauto. eauto. eauto. inversion H1. inversion H2. inversion H1. inversion H1. inversion H1.
+inv sstack; simpl in *. destruct q. simpl in *. destruct H1. destruct H. destruct H.
+destruct ( find_function m fn0) eqn:?. destruct (find_block (blks (df_instrs d0)) bk0) eqn:?.
+destruct ( block_to_cmd b0 (IId id)) eqn:?. destruct p. inv H. destruct o1. inv H0.
 
 
 
 
-
-simpl in *. eapply sound_succ_state. eapply AN.  unfold get_successors. simpl in *. rewrite Heqo0. rewrite Heqo1. rewrite Heqo2. eauto. unfold get_successors. simpl in *. unfold next_term. unfold block_entry_pc. simpl in *.  rewrite Heqo0. rewrite Heqo1. rewrite Heqo2. rewrite Heqo3. simpl. eauto. unfold transfer'. simpl in *. rewrite Heqo0. rewrite Heqo1. rewrite Heqo2. eauto. eauto. eauto.
-
-
-
-
-simpl in *. eapply sound_succ_state. eapply AN.  unfold get_successors. simpl in *. rewrite Heqo0. rewrite Heqo1. rewrite Heqo2. eauto. unfold get_successors. simpl in *. unfold next_term. unfold block_entry_pc. simpl in *.  rewrite Heqo0. rewrite Heqo1. rewrite Heqo2. rewrite Heqo3.
-destr_eq ( find_block_entry m fn br1). destr b0.
-unfold transfer'. simpl in *. rewrite Heqo0. rewrite Heqo1. rewrite Heqo2. eauto. eauto. eauto.
+eapply sound_succ_state; eauto; unfold transfer', CFG.fetch, successor_pc, fetch, cfg_to_cmd; simpl in *; try rewrite Heqo3; try rewrite Heqo4;try rewrite Heqo5; simpl in *; eauto; eapply ematch_update; eauto; try constructor. inversion H0. inversion H0. inversion H0. inversion H0.
 
 
 
 
+inv sstack; simpl in *. destruct p. simpl in *. destruct H1. destruct H. destruct H. destruct H.
+destruct H0. destruct H1.
+
+destruct ( find_function m fn0) eqn:?. destruct (find_block (blks (df_instrs d0)) bk0) eqn:?.
+destruct (  block_to_cmd b0 (IVoid x1)) eqn:?. destruct p.  destruct o1. inv H1. inv H2.
 
 
-simpl in *.  eapply sound_succ_state. eapply AN.  unfold get_successors. simpl in *. rewrite Heqo0. rewrite Heqo1. rewrite Heqo2. eauto. unfold get_successors. simpl in *. unfold next_term. unfold block_entry_pc. simpl in *.  rewrite Heqo0. rewrite Heqo1. rewrite Heqo2. rewrite Heqo3. simpl in *; eauto.
-unfold transfer'. simpl in *. rewrite Heqo0. rewrite Heqo1. rewrite Heqo2. eauto. eauto. eauto.
 
-Qed.
+
+eapply sound_succ_state; eauto; unfold transfer', CFG.fetch, successor_pc, fetch, cfg_to_cmd; simpl in *; try rewrite Heqo3; try rewrite Heqo4; try rewrite Heqo5; simpl in *; eauto. inv H2. inv H2. inv H2. inv H2.
+
+
+
+
+
+
+
+
+
+
+
+unfold jump in *. simpl in *. unfold CFG.find_block_entry in *. simpl in *. rewrite Heqo0 in Heqe1. destruct ( find_block (blks (df_instrs d)) br1) eqn:?. simpl in *. unfold monad_fold_right in *.
+
+remember ((fix
+             monad_fold_right (A B : Type) (M : Type -> Type) (H : Functor M) 
+                              (H0 : Monad) (f : A -> B -> M A) (l : seq B) 
+                              (a : A) {struct l} : M A :=
+               match l with
+               | [::] => mret a
+               | x :: xs => monad_fold_right A B M H H0 f xs a ≫= (fun y : A => f y x)
+               end)). rewrite <- Heqp in Heqe1. destruct p. simpl in *. inv Heqe1. inv Heqe1.
+
+eapply sound_succ_state; eauto; unfold transfer', CFG.fetch, successor_pc, fetch, cfg_to_cmd, find_block_pc,  CFG.find_block_entry; simpl in *; try rewrite Heqo0; try rewrite Heqo1; try rewrite Heqo2; try rewrite Heqo3; simpl in *; eauto; constructor. inv Heqe1.
+
+
+
+
+
+
+
+
+
+unfold jump in *. simpl in *. unfold CFG.find_block_entry in *. simpl in *. rewrite Heqo0 in Heqe1. destruct ( find_block (blks (df_instrs d)) br2) eqn:?. simpl in *. unfold monad_fold_right in *.
+
+remember  ((fix
+             monad_fold_right (A B : Type) (M : Type -> Type) (H : Functor M) 
+                              (H0 : Monad) (f : A -> B -> M A) (l : seq B) 
+                              (a : A) {struct l} : M A :=
+               match l with
+               | [::] => mret a
+               | x :: xs => monad_fold_right A B M H H0 f xs a ≫= (fun y : A => f y x)
+               end)). rewrite <- Heqp in Heqe1. destruct p. simpl in *. inv Heqe1. inv Heqe1.
+
+eapply sound_succ_state; eauto; unfold transfer', CFG.fetch, successor_pc, fetch, cfg_to_cmd, find_block_pc,  CFG.find_block_entry; simpl in *; try rewrite Heqo0; try rewrite Heqo1; try rewrite Heqo2; eauto. rewrite Heqo3. destruct ( find_block (blks (df_instrs d)) br1). simpl in *. eauto. simpl in *; eauto. constructor. inv Heqe1.
+
+
+
+
+
+
+
+
+
+
+
+
+
+
+unfold jump in *. simpl in *. unfold CFG.find_block_entry in *. simpl in *.
+rewrite Heqo0 in Heqe0. destruct ( find_block (blks (df_instrs d)) br) eqn:?.
+simpl in *. unfold monad_fold_right in *.
+
+remember  ((fix
+             monad_fold_right (A B : Type) (M : Type -> Type) (H : Functor M) 
+                              (H0 : Monad) (f : A -> B -> M A) (l : seq B) 
+                              (a : A) {struct l} : M A :=
+               match l with
+               | [::] => mret a
+               | x :: xs => monad_fold_right A B M H H0 f xs a ≫= (fun y : A => f y x)
+               end)). rewrite <- Heqp in Heqe0. destruct p. simpl in *. inv Heqe0. inv Heqe0.
+
+eapply sound_succ_state; eauto; unfold transfer', CFG.fetch, successor_pc, fetch, cfg_to_cmd, find_block_pc,  CFG.find_block_entry; simpl in *; try rewrite Heqo0; try rewrite Heqo1; try rewrite Heqo2; eauto.
+rewrite Heqo3. simpl in *. eauto. constructor. inv Heqe0. Qed.
