src/coq/optimisations/local_cfg.v
@@ -1,0 +1,69 @@
+Require Import Vellvm.CFG.
+Require Import Vellvm.Ollvm_ast.
+Require Import Equalities.
+
+
+
+Record local_pc : Set := mk_localpc { lbk : block_id;  lpt : instr_id }.
+
+Definition cfg_to_cmd (c:cfg) (p:local_pc) : option (cmd * option instr_id) :=
+  match find_block (blks c) (lbk p) with
+  | Some b => block_to_cmd b (lpt p) 
+  | None => None
+  end.
+
+
+Definition incr_local_pc (c:cfg) (p:local_pc) :=
+  match cfg_to_cmd c p with
+  | Some (_, Some i) => Some (mk_localpc (lbk p) i)
+  | _ => None
+  end.
+
+
+Definition fetch (c:cfg) (p:local_pc) : option cmd :=
+  match cfg_to_cmd c p with
+  | Some (instr, _) => Some instr
+  | _ => None
+  end.
+
+
+
+Definition find_block_entry (c:cfg) (b:block_id) :=
+  match find_block (blks c) b with
+  | Some block => cons (mk_localpc b (blk_entry_id block)) nil
+  | None => nil
+  end.
+
+Definition term_successor (c:cfg) (t:terminator) : list local_pc :=
+  match t with
+  | TERM_Br_1 br => find_block_entry c br
+  | TERM_Br _ br1 br2 => find_block_entry c br1 ++ find_block_entry c br2
+                                  
+| _ => nil
+end.
+
+
+Definition successor_local_pc (c:cfg) (p:local_pc) :=
+  match cfg_to_cmd c p with
+  | Some (CFG.Step ins, Some i) => cons (mk_localpc (lbk p) i) nil
+  | Some (Term t, _ ) => term_successor c t
+  | _ => nil
+  end.
+
+
+
+Module local_pcDec <: MiniDecidableType.
+  Definition t := local_pc.
+  Lemma eq_dec : forall (x y : local_pc), {x = y} + {x <> y}.
+  Proof.
+    decide equality. SearchAbout instr_id.
+    - eapply AstLib.InstrID.eq_dec.
+    -eapply AstLib.RawID.eq_dec.
+  Qed.
+  
+End  local_pcDec.
+
+
+
+Definition pc_to_local_pc (p:pc) : local_pc := mk_localpc (bk p) (pt p).
+Definition local_pc_to_pc (fn:function_id) (p:local_pc) := mk_pc fn (lbk p) (lpt p).
