src/coq/optimisations/vellvm_tactics.v
@@ -1,4 +1,24 @@
 Ltac dupl x := generalize x; intro.
 Ltac contra_destr x := remember x; destruct x; try contradiction; auto.
-Ltac save_destr x := remember x; destruct x.
 Ltac inv x := inversion x; subst; auto.
+
+
+Ltac destr_eq t := destruct t eqn:?; simpl; eauto.
+Ltac destr t := destruct t; simpl; eauto.
+Ltac appl t y := generalize y; intro; apply t in y.
+
+
+Ltac break_inner_match' t :=
+  match t with
+   | context[match ?X with _ => _ end] => break_inner_match' X || destruct X eqn:?
+   | _ => destruct t eqn:?
+ end.
+
+Ltac break_inner_match_goal :=
+  match goal with
+   | [ |- context[match ?X with _ => _ end] ] =>
+     break_inner_match' X
+ end.
+
+Ltac break_goal :=  break_inner_match_goal; simpl in *; eauto; try constructor.
+Ltac try_resolve := try (repeat break_goal); try constructor.
